src/go_lang/lang.v
@@ -108,8 +108,10 @@ Inductive prim_op : arity -> Set :=
   | LoadOp : prim_op args1
   | MapGetOp : prim_op args2 (* map loc, key *)
   | MapInsertOp : prim_op args3 (* map loc, key *)
-  | EncodeIntOp : prim_op args2 (* int, loc to store to *)
-  | DecodeIntOp : prim_op args1 (* loc to load from *)
+  | EncodeInt64Op : prim_op args2 (* int, loc to store to *)
+  | DecodeInt64Op : prim_op args1 (* loc to load from *)
+  | EncodeInt32Op : prim_op args2 (* int, loc to store to *)
+  | DecodeInt32Op : prim_op args1 (* loc to load from *)
 .
 
 Inductive expr :=
@@ -164,8 +166,10 @@ Notation Store := (Primitive2 StoreOp).
 Notation Load := (Primitive1 LoadOp).
 Notation MapGet := (Primitive2 MapGetOp).
 Notation MapInsert := (Primitive3 MapInsertOp).
-Notation EncodeInt := (Primitive2 EncodeIntOp).
-Notation DecodeInt := (Primitive1 DecodeIntOp).
+Notation EncodeInt64 := (Primitive2 EncodeInt64Op).
+Notation DecodeInt64 := (Primitive1 DecodeInt64Op).
+Notation EncodeInt32 := (Primitive2 EncodeInt32Op).
+Notation DecodeInt32 := (Primitive1 DecodeInt32Op).
 
 Fixpoint flatten_struct (v: val) : list val :=
   match v with
@@ -454,8 +458,10 @@ Proof.
                                 | LoadOp => inr 2
                                 | MapGetOp => inr 3
                                 | MapInsertOp => inr 4
-                                | EncodeIntOp => inr 5
-                                | DecodeIntOp => inr 6
+                                | EncodeInt64Op => inr 5
+                                | DecodeInt64Op => inr 6
+                                | EncodeInt32Op => inr 8
+                                | DecodeInt32Op => inr 9
                                 end)
                          (λ v, match v with
                                | inl s => a_prim_op (PanicOp s)
@@ -465,8 +471,10 @@ Proof.
                                | inr 2 => a_prim_op LoadOp
                                | inr 3 => a_prim_op MapGetOp
                                | inr 4 => a_prim_op MapInsertOp
-                               | inr 5 => a_prim_op EncodeIntOp
-                               | inr _ => a_prim_op DecodeIntOp
+                               | inr 5 => a_prim_op EncodeInt64Op
+                               | inr 6 => a_prim_op DecodeInt64Op
+                               | inr 8 => a_prim_op EncodeInt32Op
+                               | inr _ => a_prim_op DecodeInt32Op
                                end) _); by intros [_ []].
 Qed.
 
@@ -870,12 +878,12 @@ Definition map_insert (m_def: gmap u64 val * val) (k: u64) (v: val) : gmap u64 v
   let (m, def) := m_def in
   (<[ k := v ]> m, def).
 
-Definition u64_le_vals (x:u64) : list val :=
-  (λ b, LitV (LitByte b)) <$> u64_le x.
+Definition byte_vals : list byte -> list val :=
+   fmap (λ b, LitV (LitByte b)).
 
-Theorem u64_le_vals_length x : length (u64_le_vals x) = 8%nat.
+Theorem byte_vals_length bs : length (byte_vals bs) = length bs.
 Proof.
-  rewrite /u64_le_vals fmap_length u64_le_length //.
+  rewrite /byte_vals fmap_length //.
 Qed.
 
 Inductive head_step : expr → state → list observation → expr → state → list expr → Prop :=
@@ -953,19 +961,29 @@ Inductive head_step : expr → state → list observation → expr → state →
                []
                (Val v') σ'
                []
-  | EncodeIntS v l σ :
+  | EncodeInt64S v l σ :
      (forall i, (i < 8)%nat -> is_Some (σ.(heap) !! (l +ₗ i))) ->
-     head_step (EncodeInt (Val $ LitV $ LitInt v) (Val $ LitV $ LitLoc l)) σ
+     head_step (EncodeInt64 (Val $ LitV $ LitInt v) (Val $ LitV $ LitLoc l)) σ
                []
-               (Val $ LitV LitUnit) (state_insert_list l (u64_le_vals v) σ)
+               (Val $ LitV LitUnit) (state_insert_list l (byte_vals $ u64_le v) σ)
                []
-  | DecodeIntS l v σ :
-     (* TODO: this should probably be expressed in terms of bytes rather than
-     requiring a little-endian encoding *)
-     (forall i, (i < 8)%nat -> σ.(heap) !! (l +ₗ i) = u64_le_vals v !! i) ->
-     head_step (DecodeInt (Val $ LitV $ LitLoc l)) σ
+  | DecodeInt64S l vs σ :
+     (forall i, (i < 8)%nat -> σ.(heap) !! (l +ₗ i) = byte_vals vs !! i) ->
+     head_step (DecodeInt64 (Val $ LitV $ LitLoc l)) σ
                []
-               (Val $ LitV $ LitInt v) σ
+               (Val $ LitV $ LitInt (le_to_u64 vs)) σ
+               []
+  | EncodeInt32S v l σ :
+     (forall i, (i < 4)%nat -> is_Some (σ.(heap) !! (l +ₗ i))) ->
+     head_step (EncodeInt32 (Val $ LitV $ LitInt32 v) (Val $ LitV $ LitLoc l)) σ
+               []
+               (Val $ LitV LitUnit) (state_insert_list l (byte_vals $ u32_le v) σ)
+               []
+  | DecodeInt32S l vs σ :
+     (forall i, (i < 8)%nat -> σ.(heap) !! (l +ₗ i) = byte_vals vs !! i) ->
+     head_step (DecodeInt32 (Val $ LitV $ LitLoc l)) σ
+               []
+               (Val $ LitV $ LitInt32 (le_to_u32 vs)) σ
                []
   | CmpXchgS l v1 v2 vl σ b :
      σ.(heap) !! l = Some vl →
@@ -1100,5 +1118,7 @@ Notation Store := (Primitive2 StoreOp).
 Notation Load := (Primitive1 LoadOp).
 Notation MapGet := (Primitive2 MapGetOp).
 Notation MapInsert := (Primitive3 MapInsertOp).
-Notation EncodeInt := (Primitive2 EncodeIntOp).
-Notation DecodeInt := (Primitive1 DecodeIntOp).
+Notation EncodeInt64 := (Primitive2 EncodeInt64Op).
+Notation DecodeInt64 := (Primitive1 DecodeInt64Op).
+Notation EncodeInt32 := (Primitive2 EncodeInt32Op).
+Notation DecodeInt32 := (Primitive1 DecodeInt32Op).
