src/go_lang/slice.v
@@ -173,7 +173,7 @@ Admitted.
 
 Definition UInt64Put: val :=
   λ: "p" "n",
-  EncodeInt "n" (slice.ptr "p").
+  EncodeInt64 "n" (slice.ptr "p").
 
 Theorem UInt64Put_t : ⊢ UInt64Put : (slice.T byteT -> uint64T -> unitT).
 Proof.
@@ -182,9 +182,27 @@ Qed.
 
 Definition UInt64Get: val :=
   λ: "p",
-  DecodeInt (slice.ptr "p").
+  DecodeInt64 (slice.ptr "p").
 
 Theorem UInt64Get_t : ⊢ UInt64Get : (slice.T byteT -> uint64T).
+Proof.
+  typecheck.
+Qed.
+
+Definition UInt32Put: val :=
+  λ: "p" "n",
+  EncodeInt32 "n" (slice.ptr "p").
+
+Theorem UInt32Put_t : ⊢ UInt32Put : (slice.T byteT -> uint32T -> unitT).
+Proof.
+  typecheck.
+Qed.
+
+Definition UInt32Get: val :=
+  λ: "p",
+  DecodeInt32 (slice.ptr "p").
+
+Theorem UInt32Get_t : ⊢ UInt32Get : (slice.T byteT -> uint32T).
 Proof.
   typecheck.
 Qed.
@@ -196,4 +214,5 @@ Global Opaque slice.T raw_slice SliceAppend SliceAppendSlice.
 Hint Resolve raw_slice_t NewSlice_t
      SliceTake_t SliceSkip_t SliceSubslice_t SliceGet_t SliceSet_t
      SliceAppend_t SliceAppendSlice_t
-     UInt64Put_t UInt64Get_t : types.
+     UInt64Put_t UInt64Get_t
+     UInt32Put_t UInt32Get_t : types.
